prove that HML definitions are equivalent for most of the subsets

HML_definitions.thy
@@ -6,6 +6,37 @@ inductive hml_trace :: "('a, 's)hml \<Rightarrow> bool" where
 "hml_trace TT" |
 "hml_trace (hml_pos \<alpha> \<phi>)" if "hml_trace \<phi>"
 
+inductive hml_failure :: "('a, 's)hml \<Rightarrow> bool"
+  where
+failure_tt: "hml_failure TT" |
+failure_pos: "hml_failure (hml_pos \<alpha> \<phi>)" if "hml_failure \<phi>" |
+failure_conj: "hml_failure (hml_conj I J \<psi>s)" 
+if "I = {}" "(\<forall>j \<in> J. (\<exists>\<alpha>. ((\<psi>s j) = hml_pos \<alpha> TT)) \<or> \<psi>s j = TT)" 
+
+inductive hml_readiness :: "('a, 's)hml \<Rightarrow> bool"
+  where
+read_tt: "hml_readiness TT" |
+read_pos: "hml_readiness (hml_pos \<alpha> \<phi>)" if "hml_readiness \<phi>"|
+read_conj: "hml_readiness (hml_conj I J \<Phi>)" 
+if "\<forall>x \<in> (\<Phi> ` (I \<union> J)). (\<exists>\<alpha>. x = (hml_pos \<alpha> TT::('a, 's)hml)) \<or> x = TT"
+
+inductive hml_impossible_futures ::  "('a, 's)hml \<Rightarrow> bool"
+  where
+  if_tt: "hml_impossible_futures TT" |
+  if_pos: "hml_impossible_futures (hml_pos \<alpha> \<phi>)" if "hml_impossible_futures \<phi>" |
+if_conj: "hml_impossible_futures (hml_conj I J \<Phi>)"
+if "I = {}" "\<forall>x \<in> (\<Phi> ` J). (hml_trace x)"
+
+inductive hml_possible_futures :: "('a, 's)hml \<Rightarrow> bool"
+  where
+pf_tt: "hml_possible_futures TT" |
+pf_pos: "hml_possible_futures (hml_pos \<alpha> \<phi>)" if "hml_possible_futures \<phi>" |
+pf_conj: "hml_possible_futures (hml_conj I J \<Phi>)" 
+if "\<forall>x \<in> (\<Phi> ` (I\<union> J)). (hml_trace x)"
+
+definition hml_possible_futures_formulas where
+"hml_possible_futures_formulas \<equiv> {\<phi>. hml_possible_futures \<phi>}"
+
 inductive hml_failure_trace :: "('a, 's)hml \<Rightarrow> bool" where
 "hml_failure_trace TT" |
 "hml_failure_trace (hml_pos \<alpha> \<phi>)" if "hml_failure_trace \<phi>" |
@@ -13,10 +44,32 @@ inductive hml_failure_trace :: "('a, 's)hml \<Rightarrow> bool" where
   if "(\<Phi> ` I) = {} \<or> (\<exists>i \<in> \<Phi> ` I. \<Phi> ` I = {i} \<and> hml_failure_trace i)"
      "\<forall>j \<in> \<Phi> ` J. \<exists>\<alpha>. j = (hml_pos \<alpha> TT) \<or> j = TT" 
 
+inductive hml_ready_trace :: "('a, 's)hml \<Rightarrow> bool"
+  where
+r_trace_tt: "hml_ready_trace TT" |
+r_trace_pos: "hml_ready_trace (hml_pos \<alpha> \<phi>)" if "hml_ready_trace \<phi>"|
+r_trace_conj: "hml_ready_trace (hml_conj I J \<Phi>)" 
+if "(\<exists>x \<in> (\<Phi> ` I). hml_ready_trace x \<and> (\<forall>y \<in> (\<Phi> ` I). x \<noteq> y \<longrightarrow> (\<exists>\<alpha>. y = (hml_pos \<alpha> TT))))
+\<or> (\<forall>y \<in> (\<Phi> ` I).(\<exists>\<alpha>. y = (hml_pos \<alpha> TT)))"
+"(\<forall>y \<in> (\<Phi> ` J). (\<exists>\<alpha>. y = (hml_pos \<alpha> TT)))"
+
+inductive hml_ready_sim :: "('a, 's) hml \<Rightarrow> bool"
+  where
+"hml_ready_sim TT" |
+"hml_ready_sim (hml_pos \<alpha> \<phi>)" if "hml_ready_sim \<phi>" |
+"hml_ready_sim (hml_conj I J \<Phi>)" if 
+"(\<forall>x \<in> (\<Phi> ` I). hml_ready_sim x) \<and> (\<forall>y \<in> (\<Phi> ` J). (\<exists>\<alpha>. y = (hml_pos \<alpha> TT)))"
+
+inductive hml_2_nested_sim :: "('a, 's) hml \<Rightarrow> bool" 
+  where
+"hml_2_nested_sim TT" |
+"hml_2_nested_sim (hml_pos \<alpha> \<phi>)" if "hml_2_nested_sim \<phi>" |
+"hml_2_nested_sim (hml_conj I J \<Phi>)" 
+if "(\<forall>x \<in> (\<Phi> ` I). hml_2_nested_sim x) \<and> (\<forall>y \<in> (\<Phi> ` J). HML_simulation y)"
 
 context lts begin 
 
-lemma 
+lemma alt_trace_def_implies_trace_def:
   fixes \<phi> :: "('a, 's) hml"
   assumes "hml_trace \<phi>"
   shows "\<exists>\<psi>. HML_trace \<psi> \<and> (\<forall>s. (s \<Turnstile> \<phi>) \<longleftrightarrow> (s \<Turnstile> \<psi>))"
@@ -26,7 +79,7 @@ proof(induction \<phi> rule: hml_trace.induct)
   then show ?case using trace_tt by blast
 next
   case (2 \<phi> \<alpha>)
-then obtain \<psi> where "HML_trace \<psi>" and IH: "(\<forall>s. (s \<Turnstile> \<phi>) = (s \<Turnstile> \<psi>))" by blast
+  then obtain \<psi> where "HML_trace \<psi>" and IH: "(\<forall>s. (s \<Turnstile> \<phi>) = (s \<Turnstile> \<psi>))" by blast
   hence "HML_trace (hml_pos \<alpha> \<psi>)" 
     by (simp add: trace_pos)
   have "(\<forall>s. (s \<Turnstile> hml_pos \<alpha> \<phi>) = (s \<Turnstile> (hml_pos \<alpha> \<psi>)))" using IH 
@@ -35,7 +88,7 @@ then obtain \<psi> where "HML_trace \<psi>" and IH: "(\<forall>s. (s \<Turnstile
     using \<open>HML_trace (hml_pos \<alpha> \<psi>)\<close> by blast
 qed
 
-lemma 
+lemma trace_def_implies_alt_trace_def:
   fixes \<phi> :: "('a, 's) hml"
   assumes "HML_trace \<phi>"
   shows "\<exists>\<psi>. hml_trace \<psi> \<and> (\<forall>s. (s \<Turnstile> \<phi>) \<longleftrightarrow> (s \<Turnstile> \<psi>))"
@@ -60,7 +113,334 @@ next
     by blast
 qed
 
-lemma 
+lemma trace_definitions_equivalent: 
+  "\<forall>\<phi>. (HML_trace \<phi> \<longrightarrow> (\<exists>\<psi>. hml_trace \<psi> \<and> (s \<Turnstile> \<psi> \<longleftrightarrow> s \<Turnstile> \<phi>)))"
+  "\<forall>\<phi>. (hml_trace \<phi> \<longrightarrow> (\<exists>\<psi>. HML_trace \<psi> \<and> (s \<Turnstile> \<psi> \<longleftrightarrow> s \<Turnstile> \<phi>)))"
+  using trace_def_implies_alt_trace_def alt_trace_def_implies_trace_def by blast+
+
+lemma alt_failure_def_implies_failure_def:
+  fixes \<phi> :: "('a, 's) hml"
+  assumes "hml_failure \<phi>"
+  shows "\<exists>\<psi>. HML_failure \<psi> \<and> (\<forall>s. (s \<Turnstile> \<phi>) \<longleftrightarrow> (s \<Turnstile> \<psi>))"
+  using assms proof induct
+  case failure_tt
+  then show ?case 
+    using HML_failure.failure_tt by blast
+next
+  case (failure_pos \<phi> \<alpha>)
+  then show ?case 
+    using HML_failure.failure_pos by fastforce
+next
+  case (failure_conj I J \<psi>s)
+  have "HML_failure (hml_conj I J \<psi>s)"
+    by (metis HML_failure.failure_conj TT_like.intros(1) empty_iff failure_conj.hyps(1) failure_conj.hyps(2))
+  then show ?case 
+    by blast
+qed
+
+lemma failure_def_implies_alt_failure_def:
+  fixes \<phi> :: "('a, 's) hml"
+  assumes "HML_failure \<phi>"
+  shows "\<exists>\<psi>. hml_failure \<psi> \<and> (\<forall>s. (s \<Turnstile> \<phi>) \<longleftrightarrow> (s \<Turnstile> \<psi>))"
+  using assms proof(induct)
+  case failure_tt
+  then show ?case 
+    using hml_failure.failure_tt by blast
+next
+  case (failure_pos \<phi> \<alpha>)
+  then obtain \<psi> where "hml_failure \<psi>" "(\<forall>s. (s \<Turnstile> \<phi>) = (s \<Turnstile> \<psi>))" by blast
+  hence "hml_failure (hml_pos \<alpha> \<psi>) \<and> (\<forall>s. (s \<Turnstile> hml_pos \<alpha> \<phi>) = (s \<Turnstile> (hml_pos \<alpha> \<psi>)))" 
+    by (simp add: hml_failure.failure_pos)
+  then show ?case by blast
+next
+  case (failure_conj I \<psi>s J)
+  then show ?case proof(cases "\<not>(\<exists>j \<in> J. TT_like (\<psi>s j)) \<and> \<psi>s ` I \<inter> \<psi>s ` J = {}")
+    case True
+    hence "\<forall>j \<in> J. (\<exists>\<alpha> \<chi>. \<psi>s j = hml_pos \<alpha> \<chi> \<and> TT_like \<chi>)" 
+      using local.failure_conj by blast
+    define \<Psi> where "\<Psi> \<equiv> (\<lambda>i. (if i \<in> J
+                          then (hml_pos (SOME \<alpha>. \<exists>\<chi>. \<psi>s i = hml_pos \<alpha> \<chi> \<and> TT_like \<chi>) TT)::('a, 's)hml 
+                          else undefined))"
+    hence "\<forall>\<psi> \<in> \<Psi> ` J. \<exists>\<alpha>. \<psi> = hml_pos \<alpha> TT" 
+      by force
+    hence "\<forall>j \<in> J. \<exists>\<alpha> \<chi>. \<psi>s j = hml_pos \<alpha> \<chi> \<and> TT_like \<chi> \<and> \<Psi> j = hml_pos \<alpha> TT" 
+      using \<Psi>_def \<open>\<forall>j\<in>J. \<exists>\<alpha> \<chi>. \<psi>s j = hml_pos \<alpha> \<chi> \<and> TT_like \<chi>\<close> by fastforce
+    hence "(\<forall>s. \<forall>j \<in> J. (\<not>(s \<Turnstile> (\<Psi> j)) = (\<not>(s \<Turnstile> (\<psi>s j)))))" 
+      using True HML_true_TT_like HML_true_def by auto
+    have "\<forall>s. \<forall>i \<in> I. s \<Turnstile> \<psi>s i" 
+      using HML_true_TT_like HML_true_def local.failure_conj by blast
+    hence "(\<forall>s. (s \<Turnstile> hml_conj I J \<psi>s) = (s \<Turnstile> (hml_conj {} J \<Psi>)))"
+      using \<open>(\<forall>s. \<forall>j \<in> J. (\<not>(s \<Turnstile> (\<Psi> j)) = (\<not>(s \<Turnstile> (\<psi>s j)))))\<close>
+      by simp
+    have "hml_failure (hml_conj {} J \<Psi>)" 
+      using \<Psi>_def hml_failure.failure_conj
+      by (metis (no_types, lifting))
+    then show ?thesis 
+      using \<open>\<forall>s. (s \<Turnstile> hml_conj I J \<psi>s) = (s \<Turnstile> hml_conj {} J \<Psi>)\<close> by blast
+  next
+    case False
+    hence "\<forall>s. \<not>(s \<Turnstile> hml_conj I J \<psi>s)" 
+      using HML_true_TT_like HML_true_def by fastforce
+    from False obtain \<phi> i_\<phi> where "\<phi> \<in> \<psi>s ` I \<inter> \<psi>s ` J \<or> (\<phi> \<in> \<psi>s ` J \<and> TT_like \<phi>)" "\<psi>s i_\<phi> = \<phi>"
+      by blast
+    define \<Psi> where "\<Psi> \<equiv> (\<lambda>i. (if i = i_\<phi> then TT::('a, 's)hml else undefined))"
+    hence "\<forall>s. \<not>(s \<Turnstile> (hml_conj {} {i_\<phi>} \<Psi>))" 
+      by auto
+    have "hml_failure (hml_conj {} {i_\<phi>} \<Psi>)" 
+      by (simp add: \<Psi>_def hml_failure.failure_conj)
+    then show ?thesis 
+      using \<open>\<forall>s. \<not> s \<Turnstile> hml_conj I J \<psi>s\<close> \<open>\<forall>s. \<not> s \<Turnstile> hml_conj {} {i_\<phi>} \<Psi>\<close> by blast
+  qed
+qed
+
+lemma failure_definitions_equivalent: 
+  "\<forall>\<phi>. (HML_failure \<phi> \<longrightarrow> (\<exists>\<psi>. hml_failure \<psi> \<and> (s \<Turnstile> \<psi> \<longleftrightarrow> s \<Turnstile> \<phi>)))"
+  "\<forall>\<phi>. (hml_failure \<phi> \<longrightarrow> (\<exists>\<psi>. HML_failure \<psi> \<and> (s \<Turnstile> \<psi> \<longleftrightarrow> s \<Turnstile> \<phi>)))"
+  using failure_def_implies_alt_failure_def alt_failure_def_implies_failure_def by blast+
+
+lemma alt_readiness_def_implies_readiness_def:
+  fixes \<phi> :: "('a, 's) hml"
+  assumes "hml_readiness \<phi>"
+  shows "\<exists>\<psi>. HML_readiness \<psi> \<and> (\<forall>s. (s \<Turnstile> \<phi>) \<longleftrightarrow> (s \<Turnstile> \<psi>))"
+  using assms proof induct
+  case read_tt
+  then show ?case 
+    using HML_readiness.read_tt by blast
+next
+  case (read_pos \<phi> \<alpha>)
+  then show ?case 
+    using HML_readiness.read_pos by fastforce
+next
+  case (read_conj \<Phi> I J)
+  hence "HML_readiness (hml_conj I J \<Phi>)" 
+    by (metis HML_readiness.read_conj TT_like.simps)
+  then show ?case by blast
+qed
+
+lemma readiness_def_implies_alt_readiness_def:
+  fixes \<phi> :: "('a, 's) hml"
+  assumes "HML_readiness \<phi>"
+  shows "\<exists>\<psi>. hml_readiness \<psi> \<and> (\<forall>s. (s \<Turnstile> \<phi>) \<longleftrightarrow> (s \<Turnstile> \<psi>))"
+  using assms proof(induct)
+  case read_tt
+  then show ?case 
+    using hml_readiness.read_tt by blast
+next
+  case (read_pos \<phi> \<alpha>)
+  then obtain \<psi> where "hml_readiness \<psi>" "(\<forall>s. (s \<Turnstile> \<phi>) = (s \<Turnstile> \<psi>))" by blast
+  hence "hml_readiness (hml_pos \<alpha> \<psi>) \<and> (\<forall>s. (s \<Turnstile> hml_pos \<alpha> \<phi>) = (s \<Turnstile> (hml_pos \<alpha> \<psi>)))"
+    by (simp add: hml_readiness.read_pos)
+  then show ?case by blast
+next
+  case (read_conj \<Phi> I J)
+  then consider "\<Phi> ` I \<inter> \<Phi> ` J = {} \<and> (\<forall>x \<in> (\<Phi> ` J). (\<exists>\<alpha> \<chi>. x = hml_pos \<alpha> \<chi> \<and> TT_like \<chi>))"
+    | "\<Phi> ` I \<inter> \<Phi> ` J \<noteq> {} \<or> (\<exists>x \<in>\<Phi>` J. (TT_like x))" 
+    by blast
+  then show ?case proof(cases)
+    case 1
+    hence "\<forall>j \<in> J. (\<exists>\<alpha> \<chi>. \<Phi> j = hml_pos \<alpha> \<chi> \<and> TT_like \<chi>)" 
+      by blast
+    define \<Psi> where "\<Psi> \<equiv> (\<lambda>i. (if (\<exists>\<alpha> \<chi>. \<Phi> i = hml_pos \<alpha> \<chi> \<and> TT_like \<chi>)
+                          then (hml_pos (SOME \<alpha>. \<exists>\<chi>. \<Phi> i = hml_pos \<alpha> \<chi> \<and> TT_like \<chi>) TT)::('a, 's)hml 
+                          else undefined))"
+    hence "\<forall>\<psi> \<in> \<Psi> ` J. \<exists>\<alpha>. \<psi> = hml_pos \<alpha> TT"
+      by (simp add: \<open>\<forall>j\<in>J. \<exists>\<alpha> \<chi>. \<Phi> j = hml_pos \<alpha> \<chi> \<and> TT_like \<chi>\<close>)
+    define I' where "I' \<equiv> {i. i \<in> I \<and> ((\<exists>\<alpha> \<chi>. \<Phi> i = hml_pos \<alpha> \<chi> \<and> TT_like \<chi>))}"
+    have "\<forall>\<psi> \<in> \<Psi> ` I'. \<exists>\<alpha>. \<psi> = hml_pos \<alpha> TT"
+      unfolding I'_def \<Psi>_def
+      by force
+    hence "\<forall>j \<in> (J \<union> I'). \<exists>\<alpha> \<chi>. \<Phi> j = hml_pos \<alpha> \<chi> \<and> TT_like \<chi> \<and> \<Psi> j = hml_pos \<alpha> TT" 
+      using \<Psi>_def \<open>\<forall>j \<in> J. (\<exists>\<alpha> \<chi>. \<Phi> j = hml_pos \<alpha> \<chi> \<and> TT_like \<chi>)\<close> 
+      unfolding \<Psi>_def I'_def
+      by force
+    hence "(\<forall>s. \<forall>j \<in> J \<union> I'. (\<not>(s \<Turnstile> (\<Psi> j)) = (\<not>(s \<Turnstile> (\<Phi> j)))))" 
+      using HML_true_TT_like HML_true_def 
+      by (metis hml_sem_pos hml_sem_tt)
+    have "\<forall>x \<in> (I - I'). TT_like (\<Phi> x)"
+      using read_conj 1
+      unfolding I'_def
+      by auto
+    hence "(\<forall>s. (s \<Turnstile> hml_conj I J \<Phi>) = (s \<Turnstile> (hml_conj I' J \<Phi>)))"
+      using HML_true_TT_like read_conj 1
+      unfolding I'_def HML_true_def 
+      by (smt (verit, del_insts) Diff_iff hml_sem_conj mem_Collect_eq)
+    hence "(\<forall>s. (s \<Turnstile> hml_conj I J \<Phi>) = (s \<Turnstile> (hml_conj I' J \<Psi>)))"
+      using \<open>(\<forall>s. \<forall>j \<in> J \<union> I'. (\<not>(s \<Turnstile> (\<Psi> j)) = (\<not>(s \<Turnstile> (\<Phi> j)))))\<close>
+      by simp
+    have "hml_readiness (hml_conj I' J \<Psi>)" 
+      using \<Psi>_def I'_def
+      using hml_readiness.simps 
+      by (smt (verit, best) Un_iff \<open>\<forall>\<psi>\<in>\<Psi> ` I'. \<exists>\<alpha>. \<psi> = hml_pos \<alpha> TT\<close> \<open>\<forall>\<psi>\<in>\<Psi> ` J. \<exists>\<alpha>. \<psi> = hml_pos \<alpha> TT\<close> image_Un)
+    then show ?thesis 
+      using \<open>\<forall>s. (s \<Turnstile> hml_conj I J \<Phi>) = (s \<Turnstile> (hml_conj I' J \<Psi>))\<close> by blast
+  next
+    case 2
+    hence "\<forall>s. \<not>s \<Turnstile> (hml_conj I J \<Phi>)" 
+      using HML_true_TT_like HML_true_def by fastforce 
+    obtain \<phi> i_\<phi> where "\<phi> \<in> \<Phi> ` I \<inter> \<Phi> ` J \<or> (\<phi> \<in> \<Phi> ` J \<and> TT_like \<phi>)" "\<Phi> i_\<phi> = \<phi>"
+      using 2 by blast
+    define \<Psi> where "\<Psi> \<equiv> (\<lambda>i. (if i = i_\<phi> then TT::('a, 's)hml else undefined))"
+    have "hml_readiness (hml_conj {} {i_\<phi>} \<Psi>)" 
+      by (simp add: \<Psi>_def hml_readiness.read_conj)
+    have "\<forall>s. \<not>s \<Turnstile> (hml_conj {} {i_\<phi>} \<Psi>)" 
+      by (simp add: \<Psi>_def)
+    then show ?thesis 
+      using \<open>\<forall>s. \<not> s \<Turnstile> hml_conj I J \<Phi>\<close> \<open>hml_readiness (hml_conj {} {i_\<phi>} \<Psi>)\<close> by blast
+  qed
+qed
+
+lemma readiness_definitions_equivalent: 
+  "\<forall>\<phi>. (HML_readiness \<phi> \<longrightarrow> (\<exists>\<psi>. hml_readiness \<psi> \<and> (s \<Turnstile> \<psi> \<longleftrightarrow> s \<Turnstile> \<phi>)))"
+  "\<forall>\<phi>. (hml_readiness \<phi> \<longrightarrow> (\<exists>\<psi>. HML_readiness \<psi> \<and> (s \<Turnstile> \<psi> \<longleftrightarrow> s \<Turnstile> \<phi>)))"
+  using readiness_def_implies_alt_readiness_def alt_readiness_def_implies_readiness_def by blast+
+
+lemma alt_impossible_futures_def_implies_impossible_futures_def:
+  fixes \<phi> :: "('a, 's) hml"
+  assumes "hml_impossible_futures \<phi>"
+  shows "\<exists>\<psi>. HML_impossible_futures \<psi> \<and> (\<forall>s. (s \<Turnstile> \<phi>) \<longleftrightarrow> (s \<Turnstile> \<psi>))"
+  using assms proof induct
+  case if_tt
+  then show ?case 
+    using HML_impossible_futures.if_tt by blast
+next
+  case (if_pos \<phi> \<alpha>)
+  then show ?case 
+    using HML_impossible_futures.if_pos by fastforce
+next
+  case (if_conj I \<Phi> J)
+  then consider "\<Phi> ` I \<inter> \<Phi> ` J \<noteq> {} \<or> (\<exists>x\<in>\<Phi> ` J. x = TT)"
+    | "\<Phi> ` I \<inter> \<Phi> ` J = {} \<and> (\<forall>x\<in>\<Phi>`J. x \<noteq> TT) \<and> (\<exists>x. x \<in> \<Phi>`J)"
+    | "\<Phi> ` J = {}"
+    by blast
+  then show ?case proof(cases)
+    case 1
+    hence "\<forall>s. \<not>s \<Turnstile> (hml_conj I J \<Phi>)" 
+      using HML_true_TT_like HML_true_def by fastforce
+    obtain \<phi> i_\<phi> where "\<phi> \<in> \<Phi> ` I \<inter> \<Phi> ` J \<or> (\<phi> \<in> \<Phi> ` J \<and> \<phi> = TT)" "\<Phi> i_\<phi> = \<phi>"
+      using 1 by blast
+    define \<Psi> where "\<Psi> \<equiv> (\<lambda>i. (if i = i_\<phi> then TT::('a, 's)hml else undefined))"
+    have "HML_impossible_futures (hml_conj {} {i_\<phi>} \<Psi>)" 
+      using \<Psi>_def HML_impossible_futures.simps trace_tt by fastforce
+   have "\<forall>s. \<not>s \<Turnstile> (hml_conj {} {i_\<phi>} \<Psi>)"
+      by (simp add: \<Psi>_def)
+    then show ?thesis 
+      using \<open>\<forall>s. \<not> s \<Turnstile> hml_conj I J \<Phi>\<close> \<open>HML_impossible_futures (hml_conj {} {i_\<phi>} \<Psi>)\<close> by blast
+  next
+    case 2
+    hence "\<forall>x \<in> \<Phi>`J. \<exists>\<alpha> \<phi>. x = (hml_pos \<alpha> \<phi>) \<and> hml_trace \<phi>"
+      using if_conj 
+      by (meson hml_trace.cases)
+    hence "\<forall>x \<in> \<Phi>`J. \<exists>\<alpha> \<phi>. x = (hml_pos \<alpha> \<phi>) \<and> hml_trace \<phi> \<and> (\<exists>\<psi>. HML_trace \<psi> \<and> (\<forall>s. s \<Turnstile> \<phi> \<longleftrightarrow> s \<Turnstile> \<psi>))"
+      using alt_trace_def_implies_trace_def by meson
+    hence SOME_ex: "\<forall>j \<in> J. \<exists>\<alpha>. (\<exists>\<phi>. \<Phi> j = hml_pos \<alpha> \<phi>) \<and> (\<exists>\<psi>. \<exists>\<phi>. \<Phi> j = hml_pos \<alpha> \<phi> \<and> HML_trace \<psi> \<and> (\<forall>s. s \<Turnstile> \<phi> \<longleftrightarrow> s \<Turnstile> \<psi>))"
+      by (meson imageI)
+    hence SOME_all: "\<forall>j \<in> J. \<forall>\<alpha> \<phi>. \<Phi> j = hml_pos \<alpha> \<phi> \<longrightarrow> (\<exists>\<psi>. HML_trace \<psi> \<and> (\<forall>s. s \<Turnstile> \<phi> \<longleftrightarrow> s \<Turnstile> \<psi>))"
+      by fastforce
+    define \<Psi> where "\<Psi> \<equiv> (\<lambda>i. (if i \<in> J
+    then (hml_pos (SOME \<alpha>. \<exists>\<phi>. \<Phi> i = hml_pos \<alpha> \<phi>) 
+      (SOME \<psi>. \<exists>\<alpha> \<phi>. \<Phi> i = hml_pos \<alpha> \<phi> \<and> HML_trace \<psi> \<and> (\<forall>s. s \<Turnstile> \<phi> \<longleftrightarrow> s \<Turnstile> \<psi>))) 
+    else undefined))"
+    hence "\<forall>j \<in> J. \<exists>\<alpha> \<psi>. \<Psi> j = hml_pos \<alpha> \<psi>"
+      using SOME_ex 
+      by simp
+    have "\<forall>j \<in> J. \<exists>\<alpha> \<phi>. \<Phi> j = hml_pos \<alpha> \<phi> \<and> (\<exists>\<psi>. HML_trace \<psi> \<and> (\<forall>s. s \<Turnstile> \<phi> \<longleftrightarrow> s \<Turnstile> \<psi>))"
+      using SOME_ex by blast
+    have "\<forall>j \<in> J. \<exists>\<alpha> \<phi>. \<Phi> j = hml_pos \<alpha> \<phi> \<and> (\<exists>\<psi>. \<exists>\<alpha> \<phi>. \<Phi> j = hml_pos \<alpha> \<phi> \<and> HML_trace \<psi> \<and> (\<forall>s. s \<Turnstile> \<phi> \<longleftrightarrow> s \<Turnstile> \<psi>))"
+      using SOME_ex by blast
+    have "\<forall>j \<in> J. \<forall>\<alpha> \<phi> \<psi>. \<Phi> j = hml_pos \<alpha> \<phi> \<and> \<Phi> j = \<psi> \<longrightarrow> \<psi> = hml_pos \<alpha> \<phi>" 
+      by blast
+    from SOME_all have "\<forall>j \<in> J. \<exists>\<alpha> \<psi>. \<Psi> j = hml_pos \<alpha> \<psi> \<and> HML_trace \<psi>"
+      using SOME_all \<Psi>_def SOME_ex someI_ex 
+      by (smt (verit, best)) 
+    hence "\<forall>j \<in> J. \<exists>\<alpha> \<psi> \<phi>. \<Psi> j = hml_pos \<alpha> \<psi> \<and> HML_trace \<psi> \<and> \<Phi> j = hml_pos \<alpha> \<phi>"
+      using SOME_ex \<Psi>_def by fastforce 
+    have "\<forall>j \<in> J. \<exists>\<alpha> \<phi>. \<Phi> j = hml_pos \<alpha> \<phi> \<and> (\<forall>\<psi>. \<psi> \<noteq> (hml_pos \<alpha> \<phi>) \<longrightarrow> \<Phi> j \<noteq> \<psi>)" 
+      using SOME_ex by blast
+
+    have "\<And>j. j \<in> J \<Longrightarrow> \<exists>\<alpha> \<psi> \<phi>. \<Psi> j = hml_pos \<alpha> \<psi> \<and> HML_trace \<psi> \<and> \<Phi> j = hml_pos \<alpha> \<phi> \<and> (\<forall>s. s \<Turnstile> \<phi> \<longleftrightarrow> s \<Turnstile> \<psi>)"
+    proof -
+      {
+        fix j assume j_in_J: "j \<in> J"
+        then show "\<exists>\<alpha> \<psi> \<phi>. \<Psi> j = hml_pos \<alpha> \<psi> \<and> HML_trace \<psi> \<and> \<Phi> j = hml_pos \<alpha> \<phi> \<and> (\<forall>s. (s \<Turnstile> \<phi>) = (s \<Turnstile> \<psi>))"
+        proof-
+        have "\<Psi> j = (if j \<in> J 
+                    then (hml_pos (SOME \<alpha>. \<exists>\<phi>. \<Phi> j = hml_pos \<alpha> \<phi>) 
+                              (SOME \<psi>. \<exists>\<alpha> \<phi>. \<Phi> j = hml_pos \<alpha> \<phi> \<and> HML_trace \<psi> \<and> (\<forall>s. s \<Turnstile> \<phi> \<longleftrightarrow> s \<Turnstile> \<psi>))) 
+                    else undefined)"
+          by (simp add: \<Psi>_def j_in_J)
+        also have "... = (hml_pos (SOME \<alpha>. \<exists>\<phi>. \<Phi> j = hml_pos \<alpha> \<phi>) 
+                              (SOME \<psi>. \<exists>\<alpha> \<phi>. \<Phi> j = hml_pos \<alpha> \<phi> \<and> HML_trace \<psi> \<and> (\<forall>s. s \<Turnstile> \<phi> \<longleftrightarrow> s \<Turnstile> \<psi>)))"
+          using j_in_J by simp
+        finally obtain \<alpha> \<phi> \<psi> where 
+          psi_def: "\<Psi> j = hml_pos \<alpha> \<psi>" and 
+          trace_psi: "HML_trace \<psi>" and 
+          phi_alpha_def: "\<Phi> j = hml_pos \<alpha> \<phi>" and
+          phi_psi_equivalence: "\<forall>s. s \<Turnstile> \<phi> \<longleftrightarrow> s \<Turnstile> \<psi>" 
+          using SOME_all \<open>\<forall>j\<in>J. \<exists>\<alpha> \<psi> \<phi>. \<Psi> j = hml_pos \<alpha> \<psi> \<and> HML_trace \<psi> \<and> \<Phi> j = hml_pos \<alpha> \<phi>\<close> hml.inject(1) j_in_J someI_ex
+          by (smt (verit, ccfv_threshold))
+        have "\<Psi> j = hml_pos \<alpha> \<psi> \<and> HML_trace \<psi> \<and> \<Phi> j = hml_pos \<alpha> \<phi> \<and> (\<forall>s. s \<Turnstile> \<phi> \<longleftrightarrow> s \<Turnstile> \<psi>)"
+          using phi_alpha_def phi_psi_equivalence psi_def trace_psi by blast
+        then show "\<exists>\<alpha> \<psi> \<phi>. \<Psi> j = hml_pos \<alpha> \<psi> \<and> HML_trace \<psi> \<and> \<Phi> j = hml_pos \<alpha> \<phi> \<and> (\<forall>s. (s \<Turnstile> \<phi>) = (s \<Turnstile> \<psi>))"
+          by blast
+      qed
+    }
+  qed
+    hence "\<forall>j \<in> J. (\<exists>\<alpha> \<psi> \<phi>. \<Psi> j = hml_pos \<alpha> \<psi> \<and> \<Phi> j = hml_pos \<alpha> \<phi> \<and> HML_trace \<psi> \<and> (\<forall>s. s \<Turnstile> \<phi> \<longleftrightarrow> s \<Turnstile> \<psi>))" 
+      using SOME_all \<Psi>_def SOME_ex someI_ex 
+      by auto
+    hence "\<forall>j \<in> J. \<forall>s. s \<Turnstile> \<Psi> j \<longleftrightarrow> s \<Turnstile> \<Phi> j"
+      using SOME_ex \<Psi>_def by fastforce
+    hence "\<forall>s. s \<Turnstile> (hml_conj I J \<Phi>) \<longleftrightarrow> s \<Turnstile> (hml_conj {} J \<Psi>)"
+      by (simp add: if_conj.hyps(1))
+    have "\<forall>j \<in> J. HML_trace (\<Psi> j)" 
+      using \<open>\<forall>j\<in>J. \<exists>\<alpha> \<psi> \<phi>. \<Psi> j = hml_pos \<alpha> \<psi> \<and> \<Phi> j = hml_pos \<alpha> \<phi> \<and> HML_trace \<psi> \<and> (\<forall>s. (s \<Turnstile> \<phi>) = (s \<Turnstile> \<psi>))\<close> trace_pos by fastforce
+    hence "HML_impossible_futures (hml_conj {} J \<Psi>)"
+      by (simp add: HML_impossible_futures.if_conj)
+    then show ?thesis 
+      using \<open>\<forall>s. (s \<Turnstile> hml_conj I J \<Phi>) = (s \<Turnstile> hml_conj {} J \<Psi>)\<close> by blast
+  next
+    case 3
+    hence "\<forall>s. s \<Turnstile> (hml_conj I J \<Phi>)" "HML_impossible_futures TT" "\<forall>s. s \<Turnstile> TT" 
+      by (simp add: if_conj.hyps(1) HML_impossible_futures.if_tt)+
+    then show ?thesis by blast
+  qed 
+qed
+
+lemma impossible_futures_def_implies_alt_impossible_futures_def:
+  fixes \<phi> :: "('a, 's) hml"
+  assumes "HML_impossible_futures \<phi>"
+  shows "\<exists>\<psi>. hml_impossible_futures \<psi> \<and> (\<forall>s. (s \<Turnstile> \<phi>) \<longleftrightarrow> (s \<Turnstile> \<psi>))"
+  using assms proof induct
+  case if_tt
+  then show ?case 
+    using hml_impossible_futures.if_tt by blast
+next
+  case (if_pos \<phi> \<alpha>)
+  then show ?case 
+    using hml_impossible_futures.if_pos by force
+next
+  case (if_conj \<Phi> I J)
+  hence "\<forall>x \<in> \<Phi>`J. (\<exists>\<psi>. hml_trace \<psi> \<and> (\<forall>s. s \<Turnstile> x \<longleftrightarrow> s \<Turnstile> \<psi>))"
+    using trace_def_implies_alt_trace_def by blast 
+  hence "\<forall>j \<in> J. (\<exists>\<psi>. hml_trace \<psi> \<and> (\<forall>s. s \<Turnstile> \<Phi> j \<longleftrightarrow> s \<Turnstile> \<psi>))"
+    by blast
+  hence "\<And>j. j \<in> J \<Longrightarrow> \<exists>\<psi>. hml_trace \<psi> \<and> (\<forall>s. s \<Turnstile> \<Phi> j \<longleftrightarrow> s \<Turnstile> \<psi>)" by blast
+  define \<Psi> where "\<Psi> \<equiv> (\<lambda>i. (if i \<in> J then (SOME \<psi>. hml_trace \<psi> \<and> (\<forall>s. s \<Turnstile> \<Phi> i \<longleftrightarrow> s \<Turnstile> \<psi>)) 
+                              else undefined))"
+  have "\<And>j. j \<in> J \<Longrightarrow> hml_trace (\<Psi> j) \<and> (\<forall>s. s \<Turnstile> \<Phi> j \<longleftrightarrow> s \<Turnstile> \<Psi> j)"
+    unfolding \<Psi>_def using \<open>\<And>j. j \<in> J \<Longrightarrow> \<exists>\<psi>. hml_trace \<psi> \<and> (\<forall>s. s \<Turnstile> \<Phi> j \<longleftrightarrow> s \<Turnstile> \<psi>)\<close>
+    by (smt (verit, ccfv_SIG) someI)
+  hence "\<forall>j \<in> J. hml_trace (\<Psi> j) \<and> (\<forall>s. s \<Turnstile> \<Phi> j \<longleftrightarrow> s \<Turnstile> \<Psi> j)" 
+    by blast
+  hence "hml_impossible_futures (hml_conj {} J \<Psi>)" 
+    using hml_impossible_futures.simps by fastforce
+  have "\<forall>s. s \<Turnstile> (hml_conj I J \<Phi>) \<longleftrightarrow> s \<Turnstile> (hml_conj {} J \<Psi>)" 
+    using HML_true_TT_like HML_true_def \<open>\<forall>j \<in> J. hml_trace (\<Psi> j) \<and> (\<forall>s. s \<Turnstile> \<Phi> j \<longleftrightarrow> s \<Turnstile> \<Psi> j)\<close> if_conj.hyps(1) by auto
+  then show ?case 
+    using \<open>hml_impossible_futures (hml_conj {} J \<Psi>)\<close> by blast
+qed
+
+lemma alt_failure_trace_def_implies_failure_trace_def:
   fixes \<phi> :: "('a, 's) hml"
   assumes "hml_failure_trace \<phi>"
   shows "\<exists>\<psi>. HML_failure_trace \<psi> \<and> (\<forall>s. (s \<Turnstile> \<phi>) \<longleftrightarrow> (s \<Turnstile> \<psi>))"
@@ -81,65 +461,71 @@ next
   case (3 \<Phi> I J)
   hence neg_case: "\<forall>j\<in>\<Phi> ` J. stacked_pos_conj_pos j" 
     using stacked_pos_conj_pos.simps nested_empty_pos_conj.intros(1) by auto
-  from 3(1) show ?case proof(rule disjE)
-    assume "\<Phi> ` I = {}"
-    hence "HML_failure_trace (hml_conj I J \<Phi>) \<and> (\<forall>s. (s \<Turnstile> hml_conj I J \<Phi>) = (s \<Turnstile> (hml_conj I J \<Phi>)))"
-      using neg_case 
-      by (simp add: f_trace_conj)
-    then show ?thesis by blast
-  next
-    assume "\<exists>i\<in>\<Phi> ` I.
-       \<Phi> ` I = {i} \<and> hml_failure_trace i \<and> (\<exists>\<psi>. HML_failure_trace \<psi> \<and> (\<forall>s. (s \<Turnstile> i) = (s \<Turnstile> \<psi>)))"
-    then obtain i \<psi> where IH: "i\<in>\<Phi> ` I" "\<Phi> ` I = {i}" "hml_failure_trace i" "HML_failure_trace \<psi>" "(\<forall>s. (s \<Turnstile> i) = (s \<Turnstile> \<psi>))"
-      by blast
-    then show ?case
-    proof(cases "I \<inter> J = {}")
-      case True
-      define \<Psi> where  \<Psi>_def: "\<Psi> = (\<lambda>x. if x \<in> I then \<psi> else (if x \<in> J then \<Phi> x else undefined))"
-      have "\<Psi> ` I = {\<psi>}" unfolding \<Psi>_def using \<open>\<Phi> ` I = {i}\<close> by auto
-      hence pos: "(\<exists>\<psi> \<in> (\<Psi> ` I). (HML_failure_trace \<psi>) \<and> (\<forall>y \<in> (\<Psi> ` I). \<psi> \<noteq> y \<longrightarrow> nested_empty_conj y))"
-        by (simp add: \<open>HML_failure_trace \<psi>\<close>)
-      hence "\<forall>\<psi> \<in> \<Psi> ` J. stacked_pos_conj_pos \<psi>"
-        unfolding \<Psi>_def
-        using neg_case \<open>I \<inter> J = {}\<close> 
-        by auto
-      hence "HML_failure_trace (hml_conj I J \<Psi>)" using pos 
-        by (simp add: f_trace_conj)
-      from \<Psi>_def have "(\<forall>s. \<forall>j \<in> J. (\<not>(s \<Turnstile> (\<Psi> j)) = (\<not>(s \<Turnstile> (\<Phi> j)))))" using IH 
-        using True by auto
-      from \<Psi>_def have "(\<forall>s. \<forall>i \<in> I. (\<not>(s \<Turnstile> (\<Psi> i)) = (\<not>(s \<Turnstile> (\<Phi> i)))))" using IH 
-        by (metis emptyE imageI insertE)
-      have "(\<forall>s. (s \<Turnstile> hml_conj I J \<Phi>) = (s \<Turnstile> (hml_conj I J \<Psi>)))" using IH hml_sem_conj \<Psi>_def 
-        using \<open>\<forall>s. \<forall>i\<in>I. (s \<Turnstile> \<Psi> i) \<noteq> (\<not> s \<Turnstile> \<Phi> i)\<close> by auto
-    then show ?thesis using \<open>HML_failure_trace (hml_conj I J \<Psi>)\<close> by blast
-    next
-      case False
-      then obtain j where "j \<in> I \<inter> J" by blast
-      from False have "(\<forall>s. \<not>(s \<Turnstile> hml_conj I J \<Phi>))"
-        using index_sets_conj_disjunct 
-        by presburger
-      define \<Psi> where "\<Psi> = (\<lambda>x. if x \<in> (I \<inter> J) then TT::('a, 's) hml else undefined)"
-      with \<open>j \<in> I \<inter> J\<close> have "\<Psi> ` (I \<inter> J) = {TT}" 
-        by auto
-      have "stacked_pos_conj_pos TT" 
-        using stacked_pos_conj_pos.intros(1) by blast
-      hence "(\<forall>y \<in> (\<Psi> ` (I \<inter> J)). stacked_pos_conj_pos y)" using \<Psi>_def \<open>j \<in> I \<inter> J\<close> 
-        using \<open>\<Psi> ` (I \<inter> J) = {TT}\<close> by fastforce
-      have "(\<forall>y \<in> (\<Psi> ` {}). nested_empty_conj y) \<and> (\<forall>y \<in> (\<Psi> ` (I \<inter> J)). stacked_pos_conj_pos y)" 
-        using neg_case 
-        using \<open>\<forall>y\<in>\<Psi> ` (I \<inter> J). stacked_pos_conj_pos y\<close> by blast
-      hence f_trace: "((\<exists>\<psi>\<in>(\<Psi> ` ({}::'s set)). HML_failure_trace \<psi> \<and> (\<forall>y\<in>(\<Psi> ` ({}::'s set)). \<psi> \<noteq> y \<longrightarrow> nested_empty_conj y)) \<or>
-     (\<forall>y\<in>(\<Psi> ` ({}::'s set)). nested_empty_conj y)) \<and>
-    (\<forall>y\<in>(\<Psi> ` (I \<inter> J)). stacked_pos_conj_pos y)" 
-        by fastforce 
-      define \<psi> where "\<psi> \<equiv> (hml_conj ({}::'s set) (I \<inter> J) \<Psi>)"
-      have "HML_failure_trace \<psi>" unfolding \<psi>_def using f_trace_conj f_trace 
-        by fastforce
-      have "\<forall>s. \<not> s \<Turnstile> \<psi>" 
-        using \<Psi>_def \<open>j \<in> I \<inter> J\<close> \<psi>_def by auto
-      then show ?thesis using \<open>HML_failure_trace \<psi>\<close> 
-        using \<open>\<forall>s. \<not> s \<Turnstile> hml_conj I J \<Phi>\<close> by blast
-    qed
+  consider "\<Phi> ` I = {}"
+| "(\<exists>i\<in>\<Phi> ` I.
+        \<Phi> ` I = {i} \<and> hml_failure_trace i \<and> (\<exists>\<psi>. HML_failure_trace \<psi> \<and> (\<forall>s. (s \<Turnstile> i) = (s \<Turnstile> \<psi>))))
+\<and> (\<forall>j\<in>\<Phi> ` J. \<exists>\<alpha>. j = hml_pos \<alpha> TT \<or> j = TT) \<and> I \<inter> J = {}"
+| "(\<exists>i\<in>\<Phi> ` I.
+        \<Phi> ` I = {i} \<and> hml_failure_trace i \<and> (\<exists>\<psi>. HML_failure_trace \<psi> \<and> (\<forall>s. (s \<Turnstile> i) = (s \<Turnstile> \<psi>))))
+\<and> (\<forall>j\<in>\<Phi> ` J. \<exists>\<alpha>. j = hml_pos \<alpha> TT \<or> j = TT) \<and> I \<inter> J \<noteq> {}"
+    using 3 by linarith
+then show ?case proof(cases)
+  case 1
+  hence "HML_failure_trace (hml_conj I J \<Phi>) \<and> (\<forall>s. (s \<Turnstile> hml_conj I J \<Phi>) = (s \<Turnstile> (hml_conj I J \<Phi>)))"
+    using neg_case 
+    by (simp add: f_trace_conj)
+  then show ?thesis by blast
+next
+  case 2
+  then obtain i \<psi> where IH: "i\<in>\<Phi> ` I" "\<Phi> ` I = {i}" "hml_failure_trace i" "HML_failure_trace \<psi>" "(\<forall>s. (s \<Turnstile> i) = (s \<Turnstile> \<psi>))"
+    by auto
+  define \<Psi> where  \<Psi>_def: "\<Psi> = (\<lambda>x. if x \<in> I then \<psi> else (if x \<in> J then \<Phi> x else undefined))"
+  have "\<Psi> ` I = {\<psi>}" unfolding \<Psi>_def using \<open>\<Phi> ` I = {i}\<close> by auto
+  hence pos: "(\<exists>\<psi> \<in> (\<Psi> ` I). (HML_failure_trace \<psi>) \<and> (\<forall>y \<in> (\<Psi> ` I). \<psi> \<noteq> y \<longrightarrow> nested_empty_conj y))"
+    by (simp add: \<open>HML_failure_trace \<psi>\<close>)
+  have "\<forall>\<psi> \<in> \<Psi> ` J. stacked_pos_conj_pos \<psi>"
+    unfolding \<Psi>_def
+    using neg_case 2
+    by auto
+  hence "HML_failure_trace (hml_conj I J \<Psi>)" using pos 
+    by (simp add: f_trace_conj)
+  from \<Psi>_def have "(\<forall>s. \<forall>j \<in> J. (\<not>(s \<Turnstile> (\<Psi> j)) = (\<not>(s \<Turnstile> (\<Phi> j)))))" using IH 
+    by auto
+  from \<Psi>_def have "(\<forall>s. \<forall>i \<in> I. (\<not>(s \<Turnstile> (\<Psi> i)) = (\<not>(s \<Turnstile> (\<Phi> i)))))" using IH 
+    by (metis emptyE imageI insertE)
+  have "(\<forall>s. (s \<Turnstile> hml_conj I J \<Phi>) = (s \<Turnstile> (hml_conj I J \<Psi>)))" using IH hml_sem_conj \<Psi>_def 
+    using \<open>\<forall>s. \<forall>i\<in>I. (s \<Turnstile> \<Psi> i) \<noteq> (\<not> s \<Turnstile> \<Phi> i)\<close> by auto
+  then show ?thesis using \<open>HML_failure_trace (hml_conj I J \<Psi>)\<close> by blast
+next
+  case 3
+  then obtain i \<psi> where IH: "i\<in>\<Phi> ` I" "\<Phi> ` I = {i}" "hml_failure_trace i" "HML_failure_trace \<psi>" "(\<forall>s. (s \<Turnstile> i) = (s \<Turnstile> \<psi>))"
+    by blast
+  then obtain j where "j \<in> I \<inter> J" 
+    using "3" by auto 
+  from 3 have "(\<forall>s. \<not>(s \<Turnstile> hml_conj I J \<Phi>))"
+    using index_sets_conj_disjunct 
+    by presburger
+  define \<Psi> where "\<Psi> = (\<lambda>x. if x \<in> (I \<inter> J) then TT::('a, 's) hml else undefined)"
+  with \<open>j \<in> I \<inter> J\<close> have "\<Psi> ` (I \<inter> J) = {TT}" 
+    by auto
+  have "stacked_pos_conj_pos TT" 
+    using stacked_pos_conj_pos.intros(1) by blast
+  hence "(\<forall>y \<in> (\<Psi> ` (I \<inter> J)). stacked_pos_conj_pos y)" using \<Psi>_def \<open>j \<in> I \<inter> J\<close> 
+    using \<open>\<Psi> ` (I \<inter> J) = {TT}\<close> by fastforce
+  have "(\<forall>y \<in> (\<Psi> ` {}). nested_empty_conj y) \<and> (\<forall>y \<in> (\<Psi> ` (I \<inter> J)). stacked_pos_conj_pos y)" 
+    using neg_case 
+    using \<open>\<forall>y\<in>\<Psi> ` (I \<inter> J). stacked_pos_conj_pos y\<close> by blast
+  hence f_trace: "((\<exists>\<psi>\<in>(\<Psi> ` ({}::'s set)). HML_failure_trace \<psi> \<and> (\<forall>y\<in>(\<Psi> ` ({}::'s set)). \<psi> \<noteq> y \<longrightarrow> nested_empty_conj y)) \<or>
+ (\<forall>y\<in>(\<Psi> ` ({}::'s set)). nested_empty_conj y)) \<and>
+(\<forall>y\<in>(\<Psi> ` (I \<inter> J)). stacked_pos_conj_pos y)" 
+    by fastforce 
+  define \<psi> where "\<psi> \<equiv> (hml_conj ({}::'s set) (I \<inter> J) \<Psi>)"
+  have "HML_failure_trace \<psi>" unfolding \<psi>_def using f_trace_conj f_trace 
+    by fastforce
+  have "\<forall>s. \<not> s \<Turnstile> \<psi>" 
+    using \<Psi>_def \<open>j \<in> I \<inter> J\<close> \<psi>_def by auto
+  then show ?thesis using \<open>HML_failure_trace \<psi>\<close> 
+    using \<open>\<forall>s. \<not> s \<Turnstile> hml_conj I J \<Phi>\<close> by blast
   qed
 qed
 
@@ -181,7 +567,7 @@ lemma nested_empty_conj_TT_or_FF:
   unfolding HML_true_def
   by(induction, simp, fastforce)
 
-lemma 
+lemma failure_trace_def_implies_alt_failure_trace_def:
   fixes \<phi> :: "('a, 's) hml"
   assumes "HML_failure_trace \<phi>"
   shows "\<exists>\<psi>. hml_failure_trace \<psi> \<and> (\<forall>s. (s \<Turnstile> \<phi>) \<longleftrightarrow> (s \<Turnstile> \<psi>))"
